@prefix rdf: <http://www.w3.org/1999/02/22-rdf-syntax-ns#> .
@prefix owl: <http://www.w3.org/2002/07/owl#> .
@prefix dc11: <http://purl.org/dc/elements/1.1/> .
@prefix dcterms: <http://purl.org/dc/terms/> .
@prefix cc: <http://creativecommons.org/ns#> .
@prefix rdfs: <http://www.w3.org/2000/01/rdf-schema#> .
@prefix vann: <http://purl.org/vocab/vann/> .

<https://w3id.org/polifonia/ontology/music-instrument/> a owl:Ontology ;
	owl:versionIRI <https://w3id.org/polifonia/ontology/music-instrument/1.0/> ;
	owl:imports <https://w3id.org/arco/ontology/location/1.2>, <https://w3id.org/polifonia/ontology/core/1.0>, <https://w3id.org/polifonia/ontology/music-meta/1.0/> ;
	dc11:creator "Jacopo de Berardinis"@en, "Valentina Carriero"@en, "Valentina Presutti"@en ;
	dc11:license <https://creativecommons.org/licenses/by-sa/4.0/> ;
	dcterms:license <https://creativecommons.org/licenses/by-sa/4.0/> ;
	cc:license <https://creativecommons.org/licenses/by-sa/4.0/> ;
	rdfs:comment "This ontology describes musical instruments as mediums of performance and their technical properties. Given that numerous taxonomies of instruments into groups and families exist (e.g. Hornbostel-Sachs, MIMO, MusicBrainz) and finding common categorisations is an open problem, our module provides an abstraction capable to express arbitrary classifications."@en ;
	rdfs:label "Music Instrument Ontology"@en ;
	dc11:title "Music Instrument Ontology"@en ;
	dc11:description "This ontology describes musical instruments as mediums of performance and their technical properties. Given that numerous taxonomies of instruments into groups and families exist (e.g. Hornbostel-Sachs, MIMO, MusicBrainz) and finding common categorisations is an open problem, our module provides an abstraction capable to express arbitrary classifications."@en ;
	owl:versionInfo "1.0"@en ;
	dcterms:modified "\"2023-05-19\"^^xsd:date" ;
	dcterms:issued "\"2023-04-12\"^^xsd:date" ;
	vann:preferredNamespacePrefix "mi:" ;
	vann:preferredNamespaceUri "https://w3id.org/polifonia/ontology/music-instrument/" .

<https://w3id.org/polifonia/ontology/instrument/hasBuilder> a owl:ObjectProperty ;
	rdfs:domain <https://w3id.org/polifonia/ontology/instrument/InstrumentRealization> ;
	rdfs:range <https://w3id.org/polifonia/ontology/core/Agent> ;
	rdfs:comment "The relation between an instrument realization and its builder."@en ;
	rdfs:label "has builder"@en .

<https://w3id.org/polifonia/ontology/instrument/wasBuiltAtTime> a owl:ObjectProperty ;
	rdfs:domain <https://w3id.org/polifonia/ontology/instrument/InstrumentRealization> ;
	rdfs:range <https://w3id.org/polifonia/ontology/core/TimeInterval> ;
	rdfs:comment "The relation between an instrument realization and the time interval it was built at."@en ;
	rdfs:label "was built at time"@en .

<https://w3id.org/polifonia/ontology/instrument/wasBuiltIn> a owl:ObjectProperty ;
	rdfs:domain <https://w3id.org/polifonia/ontology/instrument/InstrumentRealization> ;
	rdfs:range <https://w3id.org/polifonia/ontology/core/Place> ;
	rdfs:comment "The relation between an instrument realization and the place it was built in."@en ;
	rdfs:label "was built in"@en .

<https://w3id.org/polifonia/ontology/instrument/wasInventedAtTime> a owl:ObjectProperty ;
	rdfs:domain <https://w3id.org/polifonia/ontology/instrument/Instrument> ;
	rdfs:range <https://w3id.org/polifonia/ontology/core/TimeInterval> ;
	rdfs:comment "The relation between an instrument, intended as an information object, and the time interval it was invented at."@en ;
	rdfs:label "was invented at time"@en .

<https://w3id.org/polifonia/ontology/instrument/wasInventedBy> a owl:ObjectProperty ;
	rdfs:domain <https://w3id.org/polifonia/ontology/instrument/Instrument> ;
	rdfs:range <https://w3id.org/polifonia/ontology/core/Agent> ;
	rdfs:comment "The relation between an instrument as an information object and the agent which invented it."@en ;
	rdfs:label "was invented by"@en .

<https://w3id.org/polifonia/ontology/instrument/Instrument> a owl:Class ;
	rdfs:subClassOf <https://w3id.org/polifonia/ontology/core/InformationObject>, <https://w3id.org/polifonia/ontology/music-meta/MediumOfPerformance>, [
		rdf:type owl:Restriction ;
		owl:onProperty <https://w3id.org/polifonia/ontology/instrument/wasInventedAtTime> ;
		owl:someValuesFrom <https://w3id.org/polifonia/ontology/core/TimeInterval> ;
	], [
		rdf:type owl:Restriction ;
		owl:onProperty <https://w3id.org/polifonia/ontology/instrument/wasInventedBy> ;
		owl:someValuesFrom <https://w3id.org/polifonia/ontology/core/Agent> ;
	], [
		rdf:type owl:Restriction ;
		owl:onProperty <https://w3id.org/arco/ontology/core/hasPart> ;
		owl:allValuesFrom <https://w3id.org/polifonia/ontology/instrument/InstrumentPart> ;
	] ;
	rdfs:comment "An instrument intended as an information object (e.g. the guitar as an information object), regardless its physical realizations (e.g. the specific guitar at my place)."@en ;
	rdfs:label "Instrument"@en .

<https://w3id.org/polifonia/ontology/instrument/InstrumentPart> a owl:Class ;
	rdfs:comment "The part of an instrument."@en ;
	rdfs:label "Instrument part"@en .

<https://w3id.org/polifonia/ontology/instrument/InstrumentRealization> a owl:Class ;
	rdfs:subClassOf <https://w3id.org/polifonia/ontology/core/InformationRealization>, [
		rdf:type owl:Restriction ;
		owl:onProperty <https://w3id.org/arco/ontology/location/hasTimeIndexedTypedLocation> ;
		owl:someValuesFrom <https://w3id.org/arco/ontology/location/TimeIndexedTypedLocation> ;
	], [
		rdf:type owl:Restriction ;
		owl:onProperty <https://w3id.org/polifonia/ontology/core/hasName> ;
		owl:someValuesFrom <https://w3id.org/polifonia/ontology/core/Name> ;
	], [
		rdf:type owl:Restriction ;
		owl:onProperty <https://w3id.org/polifonia/ontology/core/realizes> ;
		owl:someValuesFrom <https://w3id.org/polifonia/ontology/instrument/Instrument> ;
	], [
		rdf:type owl:Restriction ;
		owl:onProperty <https://w3id.org/polifonia/ontology/instrument/wasBuiltIn> ;
		owl:someValuesFrom <https://w3id.org/polifonia/ontology/core/Place> ;
	] ;
	rdfs:comment "The physical realization of an instrument, intended as the information realization (e.g. the specific guitar at my place) and the information object (the guitar as an information object)."@en ;
	rdfs:label "Instrument realization"@en .

<https://w3id.org/polifonia/ontology/instrument/Voice> a owl:Class ;
	rdfs:subClassOf <https://w3id.org/polifonia/ontology/music-meta/MediumOfPerformance> ;
	rdfs:label "Voice"@en .

